TraceInclusions.v
@@ -3,9 +3,7 @@ Import ListNotations.
 Require Import Kami.Properties.
 Require Import Kami.PProperties.
 Require Import Kami.PPlusProperties.
-(*
-Properties.v:  Theorem simulationZeroAction:
-*)
+
 Theorem _StepSimulation (imp spec : Mod) (simRel : RegsT -> RegsT -> Prop)
         (initRel : forall rimp : list RegT,
             Forall2 regInit rimp (getAllRegisters imp)
@@ -340,4 +338,371 @@ Theorem _simulationZeroAction (imp spec: BaseModuleWf) (simRel: RegsT -> RegsT -
   TraceInclusion (Base imp) (Base spec).
 Proof.
   eauto using simulationZeroAction.
+Qed.
+
+Theorem _WfConcatAssoc1 (m1 m2 m3 : Mod) :
+  WfMod (ConcatMod m1 (ConcatMod m2 m3)) -> WfMod (ConcatMod (ConcatMod m1 m2) m3).
+Proof.
+  eauto using WfConcatAssoc1.
+Qed.
+
+Theorem _WfConcatAssoc2 (m1 m2 m3 : Mod) :
+  WfMod (ConcatMod (ConcatMod m1 m2) m3) -> WfMod (ConcatMod m1 (ConcatMod m2 m3)).
+Proof.
+  eauto using WfConcatAssoc2.
+Qed.
+
+Theorem _WfModBreakDownFile (m : Mod) :
+  WfMod m -> WfMod (mergeSeparatedBaseFile (fst (snd (separateMod m)))).
+Proof.
+  eauto using WfModBreakDownFile.
+Qed.
+
+Theorem _WfModBreakDownMod (m : Mod) :
+  WfMod m -> WfMod (mergeSeparatedBaseMod (snd (snd (separateMod m)))).
+Proof.
+  eauto using WfModBreakDownMod.
+Qed.
+
+Theorem _merged_WellFormed (m : Mod) :
+  WfMod m -> WfMod (mergeSeparatedMod (separateMod m)).
+Proof.
+  eauto using merged_WellFormed.
+Qed.
+
+Theorem _WfMod_getFlat (m : Mod) :
+  WfMod m -> WfMod (getFlat m).
+Proof.
+  eauto using WfMod_getFlat.
+Qed.
+
+Theorem _TraceInclusion_Merge_l (m : ModWf) :
+  TraceInclusion m (WfMergedMod m).
+Proof.
+  eauto using TraceInclusion_Merge_l.
+Qed.
+
+Theorem _TraceInclusion_Merge_r (m : ModWf) :
+  TraceInclusion (WfMergedMod m) m.
+Proof.
+  eauto using TraceInclusion_Merge_r.
+Qed.
+
+Theorem _ConcatMod_comm (m1 m2 : Mod) : 
+  WfMod (ConcatMod m1 m2) -> TraceInclusion (ConcatMod m1 m2) (ConcatMod m2 m1).
+Proof.
+  eauto using ConcatMod_comm.
+Qed.
+
+Theorem _ConcatModAssoc1 (m1 m2 m3 : Mod) :
+  WfMod (ConcatMod (ConcatMod m1 m2) m3) ->
+  TraceInclusion (ConcatMod m1 (ConcatMod m2 m3)) (ConcatMod (ConcatMod m1 m2) m3).
+Proof.
+  eauto using ConcatModAssoc1.
+Qed.
+
+Theorem _ConcatModAssoc2 (m1 m2 m3 : Mod) :
+  WfMod (ConcatMod (ConcatMod m1 m2) m3) ->
+  TraceInclusion (ConcatMod (ConcatMod m1 m2) m3) (ConcatMod m1 (ConcatMod m2 m3)).
+Proof.
+  eauto using ConcatModAssoc2.
+Qed.
+
+(*
+PPlusProperties.v:Theorem flatten_inline_remove_TraceInclusion (m : ModWf) :
+ *)
+
+Theorem _StrongPPlusTraceInclusion_PPlusTraceInclusion (m m' : BaseModule) :
+  StrongPPlusTraceInclusion m m' -> PPlusTraceInclusion m m'.
+Proof.
+  eauto using StrongPPlusTraceInclusion_PPlusTraceInclusion.
+Qed.
+
+Theorem _PPlusTraceInclusion_PTraceInclusion (m m' : BaseModule) :
+  PPlusTraceInclusion m m' -> PTraceInclusion m m'.
+Proof.
+  eauto using PPlusTraceInclusion_PTraceInclusion.
+Qed.
+
+Theorem _PPlusTraceInclusion_TraceInclusion (m m' : BaseModule) :
+  WfMod m ->
+  WfMod m' ->
+  PPlusTraceInclusion m m' ->
+  TraceInclusion m m'.
+Proof.
+  eauto using PPlusTraceInclusion_TraceInclusion.
+Qed.
+
+Theorem _TraceInclusion_inlining_Rules_r (m : BaseModule) (f : DefMethT) (rn : string):
+  In f (getMethods m) ->
+  WfMod m ->
+  TraceInclusion m (inlineSingle_Rule_BaseModule f rn m).
+Proof.
+  eauto using TraceInclusion_inlining_Rules_r.
+Qed.
+
+Theorem _TraceInclusion_inlining_Meth_r (m : BaseModule) (f : DefMethT) (gn : string) :
+  In f (getMethods m) ->
+  WfMod m ->
+  TraceInclusion m (inlineSingle_Meth_BaseModule f gn m).
+Proof.
+  eauto using TraceInclusion_inlining_Meth_r.
+Qed.
+
+Theorem _inline_meth_transform (f : DefMethT) (regs : list RegInitT)
+        (rules : list RuleT) (meths : list DefMethT):
+  WfMod (BaseMod regs rules meths) ->
+  In f meths ->
+  forall i : nat,
+    TraceInclusion (BaseMod regs rules meths)
+                   (BaseMod regs rules (transform_nth_right (inlineSingle_Meth f) i meths)).
+Proof.
+  eauto using inline_meth_transform.
+Qed.
+
+Theorem _inline_rule_transform (f : DefMethT) (regs : list RegInitT)
+        (rules : list RuleT) (meths : list DefMethT):
+  WfMod (BaseMod regs rules meths) ->
+  In f meths ->
+  forall i : nat,
+    TraceInclusion (BaseMod regs rules meths)
+                   (BaseMod regs (transform_nth_right (inlineSingle_Rule f) i rules) meths).
+Proof.
+  eauto using inline_rule_transform.
+Qed.
+
+Theorem _inline_meth_fold_right (f : DefMethT) (regs : list RegInitT)
+        (rules : list RuleT) (meths : list DefMethT):
+  WfMod (BaseMod regs rules meths) ->
+  forall xs : list nat,
+    In f meths ->
+    TraceInclusion (BaseMod regs rules meths)
+                   (BaseMod regs rules (fold_right (transform_nth_right (inlineSingle_Meth f)) meths xs)).
+Proof.
+  eauto using inline_meth_fold_right.
+Qed.
+
+Theorem _inline_rule_fold_right (f : DefMethT) (regs : list RegInitT)
+        (rules : list RuleT) (meths : list DefMethT):
+  WfMod (BaseMod regs rules meths) ->
+  forall xs : list nat,
+    In f meths ->
+    TraceInclusion (BaseMod regs rules meths)
+                   (BaseMod regs (fold_right (transform_nth_right (inlineSingle_Rule f)) rules xs) meths).
+Proof.
+  eauto using inline_rule_fold_right.
+Qed.
+
+Theorem _TraceInclusion_inline_BaseModule_rules (regs : list RegInitT) (rules : list RuleT)
+        (meths : list DefMethT) (f : DefMethT):
+  WfMod (BaseMod regs rules meths) ->
+  In f meths ->
+  TraceInclusion (BaseMod regs rules meths)
+                 (BaseMod regs (map (inlineSingle_Rule f) rules) meths).
+Proof.
+  eauto using TraceInclusion_inline_BaseModule_rules.
+Qed.
+
+Theorem _TraceInclusion_inline_BaseModule_meths (regs : list RegInitT)
+        (rules : list RuleT) (meths : list DefMethT) (f : DefMethT):
+  WfMod (BaseMod regs rules meths) ->
+  In f meths ->
+  TraceInclusion (BaseMod regs rules meths)
+                 (BaseMod regs rules (map (inlineSingle_Meth f) meths)).
+Proof.
+  eauto using TraceInclusion_inline_BaseModule_meths.
+Qed.
+
+Theorem _TraceInclusion_inline_BaseModule_all (regs : list RegInitT) (rules : list RuleT)
+        (meths : list DefMethT) (f : DefMethT):
+  WfMod (BaseMod regs rules meths) ->
+  In f meths ->
+  TraceInclusion (BaseMod regs rules meths) (inlineSingle_BaseModule f regs rules meths).
+Proof.
+  eauto using TraceInclusion_inline_BaseModule_all.
+Qed.
+
+Theorem _TraceInclusion_inlineSingle_pos_Rules (regs : list RegInitT) (rules : list RuleT)
+        (meths : list DefMethT):
+  WfMod (BaseMod regs rules meths) ->
+  forall n : nat,
+    WfMod (BaseMod regs (inlineSingle_Rules_pos meths n rules) meths) /\
+    TraceInclusion (BaseMod regs rules meths)
+                   (BaseMod regs (inlineSingle_Rules_pos meths n rules) meths).
+Proof.
+  eauto using TraceInclusion_inlineSingle_pos_Rules.
+Qed.
+
+Theorem _TraceInclusion_inlineAll_pos_Rules (regs : list RegInitT) (rules : list RuleT)
+        (meths : list DefMethT):
+  WfMod (BaseMod regs rules meths) ->
+  WfMod (BaseMod regs (inlineAll_Rules meths rules) meths) /\
+  TraceInclusion (BaseMod regs rules meths)
+                 (BaseMod regs (inlineAll_Rules meths rules) meths).
+Proof.
+  eauto using TraceInclusion_inlineAll_pos_Rules.
+Qed.
+
+Theorem _TraceInclusion_inlineSingle_pos_Meths (regs : list RegInitT) (rules : list RuleT)
+        (meths : list DefMethT):
+  WfMod (BaseMod regs rules meths) ->
+  forall n : nat,
+    WfMod (BaseMod regs rules (inlineSingle_Meths_pos meths n)) /\
+    TraceInclusion (BaseMod regs rules meths)
+                   (BaseMod regs rules (inlineSingle_Meths_pos meths n)).
+Proof.
+  eauto using TraceInclusion_inlineSingle_pos_Meths.
+Qed.
+
+Theorem _TraceInclusion_inlineAll_pos_Meths (regs : list RegInitT) (rules : list RuleT)
+        (meths : list DefMethT):
+  WfMod (BaseMod regs rules meths) ->
+  WfMod (BaseMod regs rules (inlineAll_Meths meths)) /\
+  TraceInclusion (BaseMod regs rules meths) (BaseMod regs rules (inlineAll_Meths meths)).
+Proof.
+  eauto using TraceInclusion_inlineAll_pos_Meths.
+Qed.
+
+Theorem _TraceInclusion_inlineAll_pos (regs : list RegInitT) (rules : list RuleT)
+        (meths : list DefMethT):
+  WfMod (BaseMod regs rules meths) ->
+  WfMod (inlineAll_All regs rules meths) /\
+  TraceInclusion (BaseMod regs rules meths) (inlineAll_All regs rules meths).
+Proof.
+  eauto using TraceInclusion_inlineAll_pos.
+Qed.
+
+Theorem _WfCreateHide_Mod (m : ModWf) :
+  WfMod (flatten_inline_everything m).
+Proof.
+  eauto using WfCreateHide_Mod.
+Qed.
+
+Theorem _TraceInclusion_flatten_inline_everything_r (m : ModWf) :
+  TraceInclusion m (inlined_ModWf m).
+Proof.
+  eauto using TraceInclusion_flatten_inline_everything_r.
+Qed.
+
+Theorem _inlineSingle_Rule_map_Wf {f : DefMethT} {m : ModWf} (inMeths : In f (getAllMethods m)):
+  WfMod (createHide (inlineSingle_Rule_map_BaseModule f (getFlat m)) (getHidden m)).
+Proof.
+  eauto using inlineSingle_Rule_map_Wf.
+Qed.
+
+Theorem _inlineSingle_Meth_map_Wf {m : ModWf} {f : DefMethT} (inMeths : In f (getAllMethods m)) :
+  WfMod (createHide (inlineSingle_Meth_map_BaseModule f (getFlat m)) (getHidden m)).
+Proof.
+  eauto using inlineSingle_Meth_map_Wf.
+Qed.
+
+Theorem _inlineSingle_Rule_map_TraceInclusion {m : ModWf} {f : DefMethT} (inMeths : In f (getAllMethods m)):
+  TraceInclusion m (inlineSingle_Rule_map_ModWf inMeths).
+Proof.
+  eauto using inlineSingle_Rule_map_TraceInclusion.
+Qed.
+
+Theorem _inlineSingle_Meth_map_TraceInclusion {m : ModWf}  {f : DefMethT} (inMeths : In f (getAllMethods m)) :
+  TraceInclusion m (inlineSingle_Meth_map_ModWf inMeths).
+Proof.
+  eauto using inlineSingle_Meth_map_TraceInclusion.
+Qed.
+
+Theorem _inlineSingle_Module_Wf {m : ModWf} {f : DefMethT} (inMeths : In f (getAllMethods m)) :
+  WfMod (inlineSingle_Module f m).
+Proof.
+  eauto using inlineSingle_Module_Wf.
+Qed.
+
+Theorem _inlineSingle_BaseModule_TraceInclusion {m : ModWf} {f : DefMethT}
+        (inMeths : In f (getAllMethods m)) :
+  TraceInclusion m (inlineSingle_Module_ModWf inMeths).
+Proof.
+  eauto using inlineSingle_BaseModule_TraceInclusion.
+Qed.
+
+Theorem _inlineSingle_BaseModule_nth_Meth_Wf {m : ModWf} {f : DefMethT}
+        (inMeths : In f (getAllMethods m)) (xs : list nat) :
+  WfMod
+    (createHide
+       (inlineSingle_BaseModule_nth_Meth f (getAllRegisters m) 
+                                         (getAllRules m) (getAllMethods m) xs) (getHidden m)).
+Proof.
+  eauto using inlineSingle_BaseModule_nth_Meth_Wf.
+Qed.
+
+Theorem _inlineSingle_BaseModule_nth_Meth_TraceInclusion {m : ModWf} {f : DefMethT}
+        (inMeths : In f (getAllMethods m)) (xs : list nat) :
+  TraceInclusion m (inlineSingle_BaseModule_nth_Meth_ModWf inMeths xs).
+Proof.
+  eauto using inlineSingle_BaseModule_nth_Meth_TraceInclusion.
+Qed.
+
+Theorem _inlineSingle_BaseModule_nth_Rule_Wf {m : ModWf} {f : DefMethT}
+        (inMeths : In f (getAllMethods m)) (xs : list nat) :
+  WfMod
+    (createHide
+       (inlineSingle_BaseModule_nth_Rule f (getAllRegisters m) 
+                                         (getAllRules m) (getAllMethods m) xs) (getHidden m)).
+Proof.
+  eauto using inlineSingle_BaseModule_nth_Rule_Wf.
+Qed.
+
+Theorem _inlineSingle_BaseModule_nth_Rule_TraceInclusion {m : ModWf} {f : DefMethT} (inMeths : In f (getAllMethods m)) (xs : list nat) :
+  TraceInclusion m (inlineSingle_BaseModule_nth_Rule_ModWf inMeths xs).
+Proof.
+  eauto using inlineSingle_BaseModule_nth_Rule_TraceInclusion.
+Qed.
+
+Theorem _inlineAll_Rules_Wf (m : ModWf):
+  WfMod (inlineAll_Rules_Mod m).
+Proof.
+  eauto using inlineAll_Rules_Wf.
+Qed.
+
+Theorem _inlineAll_Rules_TraceInclusion (m : ModWf) :
+  TraceInclusion m (inlineAll_Rules_ModWf m).
+Proof.
+  eauto using inlineAll_Rules_TraceInclusion.
+Qed.
+
+Theorem _inlineAll_Meths_Wf (m : ModWf) :
+  WfMod (inlineAll_Meths_Mod m).
+Proof.
+  eauto using inlineAll_Meths_Wf.
+Qed.
+
+Theorem _inlineAll_Meths_TraceInclusion (m : ModWf) :
+  TraceInclusion m (inlineAll_Meths_ModWf m).
+Proof.
+  eauto using inlineAll_Meths_TraceInclusion.
+Qed.
+
+Theorem _flatten_inline_remove_Wf (m : ModWf) :
+  WfMod (flatten_inline_remove m).
+Proof.
+  eauto using flatten_inline_remove_Wf.
+Qed.
+
+Theorem _removeHides_createHide_TraceInclusion (m : BaseModuleWf) (l : list string)
+        (subList : SubList l (map fst (getMethods m))):
+  NoSelfCallBaseModule m ->
+  TraceInclusion (removeHidesModWf m l) (createHideModWf m subList).
+Proof.
+  eauto using removeHides_createHide_TraceInclusion.
+Qed.
+
+Theorem _createHide_removeHides_TraceInclusion (m : BaseModuleWf) (l : list string)
+        (subList : SubList l (map fst (getMethods m))):
+  NoSelfCallBaseModule m ->
+  TraceInclusion (createHideModWf m subList) (removeHidesModWf m l).
+Proof.
+  eauto using createHide_removeHides_TraceInclusion.
+Qed.
+
+Theorem _flatten_inline_remove_TraceInclusion (m : ModWf) :
+  NoSelfCallBaseModule (inlineAll_All_mod m) ->
+  TraceInclusion (flatten_inline_everything m) (flatten_inline_remove_ModWf m).
+Proof.
+  eauto using flatten_inline_remove_TraceInclusion.
 Qed.
